implement cclique

Pearls/CelebrityCliques.dfy
@@ -14,13 +14,13 @@ module CelebrityCliques {
 
     predicate IsCelebrityClique<Person>(cs: set<Person>, ps: set<Person>)
     {
-        cs <= ps && forall x :: x in ps ==> (forall y :: y in cs ==> Knows(x, y) && (Knows(y, x) ==> x in cs))
+        cs != {} && cs <= ps && forall x :: x in ps ==> (forall y :: y in cs ==> Knows(x, y) && (Knows(y, x) ==> x in cs))
     }
 
     lemma CelebrityCliqueIsUnique<Person>(ps: set<Person>, cs: set<Person>, cs': set<Person>)
         requires IsCelebrityClique(cs, ps)
         requires IsCelebrityClique(cs', ps)
-        requires cs != {} && cs' != {}
+        // requires cs != {} && cs' != {}
         requires cs != cs'
         ensures false
     {
@@ -61,6 +61,43 @@ module CelebrityCliques {
             Map((ss: seq<T>) => prepend(xs[0], ss), subsetSeqs(xs[1..]))
             +
             subsetSeqs(xs[1..])
+    }
+
+    lemma subsetSeqsContains<T(==)>(xs: seq<T>)
+        requires distinct(xs)
+        ensures forall yy :: yy in subsetSeqs(xs) ==> forall y :: y in yy ==> y in xs
+    {
+        if xs == [] {
+            assert forall yy :: yy in subsetSeqs(xs) ==> forall y :: y in yy ==> y in xs;
+        }else if |xs|==1 {
+            assert forall yy :: yy in subsetSeqs(xs) ==> forall y :: y in yy ==> y in xs;
+        }else{
+            var x := xs[0];
+            assert xs == [xs[0]] + xs[1..];
+            subsetSeqsContains(xs[1..]);
+            var mapped := Map((ss: seq<T>) => prepend(xs[0], ss), subsetSeqs(xs[1..]));
+            forall mm | mm in mapped
+                ensures forall y :: y in mm ==> y in xs
+            {
+                forall y | y in mm
+                    ensures y in xs
+                {
+                    if y == x {
+                        assert x in xs;
+
+                    }else{
+                        var i :| 0 <= i < |mapped| && mapped[i] == mm;
+                        assert mapped[i] == [x]+subsetSeqs(xs[1..])[i];
+                        assert y in subsetSeqs(xs[1..])[i]; 
+                        assert subsetSeqs(xs[1..])[i] in subsetSeqs(xs[1..]);
+                        assert y in xs[1..];
+                        assert y in xs;
+
+                    }
+                }
+            }
+            assert forall yy :: yy in subsetSeqs(xs) ==> forall y :: y in yy ==> y in xs;
+        }
     }
 
     function seqSeqsToSet<T(==)>(xs: seq<T>): set<set<T>>
@@ -136,11 +173,153 @@ module CelebrityCliques {
         }
     }
 
-    function FindCCliqueNaive<Person(==)>(xs: seq<Person>): seq<seq<Person>>
+    lemma concatDifferent<T(==)>(xs: seq<T>, ys: seq<T>, x: T)
+        requires xs != ys
+        ensures [x]+xs != [x]+ys
+    {
+        if |xs| != |ys| {
+
+        }else{
+            var i :| 0 <= i < |xs| && xs[i] != ys[i];
+            assert ([x]+xs)[i+1] != ([x]+ys)[i+1];
+        }
+    }
+
+    lemma subsetSeqsDistinct<T(==)>(xs: seq<T>)
         requires distinct(xs)
+        ensures distinct(subsetSeqs(xs))
+    {
+        if xs == [] {
+
+        }else if |xs| == 1 {
+
+        }else{
+            var x := xs[0];
+            assert xs == [x] + xs[1..];
+            subsetSeqsDistinct(xs[1..]);
+            var mapped := Map((ss: seq<T>) => prepend(xs[0], ss), subsetSeqs(xs[1..]));
+            assert distinct(mapped) by {
+                forall i,k | i != k && 0 <= i <= k < |mapped|
+                    ensures mapped[i] != mapped[k]
+                {
+                    assert mapped[i] == prepend(xs[0], subsetSeqs(xs[1..])[i]);
+                    assert mapped[k] == prepend(xs[0], subsetSeqs(xs[1..])[k]);
+                    assert subsetSeqs(xs[1..])[i] != subsetSeqs(xs[1..])[k];
+                    assert mapped[i] == [x]+subsetSeqs(xs[1..])[i];
+                    assert mapped[k] == [x]+subsetSeqs(xs[1..])[k];
+                    concatDifferent(subsetSeqs(xs[1..])[i], subsetSeqs(xs[1..])[k], x);
+                    assert mapped[i] != mapped[k];
+                }
+                
+            }
+            forall xx | xx in mapped
+                ensures xx !in subsetSeqs(xs[1..])
+            {
+                assert x in xx;
+                subsetSeqsContains(xs[1..]);
+                assert forall yy :: yy in subsetSeqs(xs[1..]) ==> x !in yy;
+            }
+            distincts(mapped, subsetSeqs(xs[1..]));
+
+        }
+    }
+
+    lemma setsNotEqualPlusOne<T(==)>(ss: set<T>, yy: set<T>, x: T)
+        requires ss != yy
+        requires x !in ss
+        requires x !in yy
+        ensures {x}+ss != {x}+yy
+    {}
+
+    lemma subsetSeqToSetNotEqual<T(==)>(xs: seq<T>)
+        requires distinct(xs)
+        ensures forall i,j :: i != j && 0 <= i < |subsetSeqs(xs)| && 0 <= j < |subsetSeqs(xs)| ==> ToSet(subsetSeqs(xs)[i]) != ToSet(subsetSeqs(xs)[j])
+    {
+        if |xs| <= 1 {
+
+            assert forall i,j :: i != j && 0 <= i < |subsetSeqs(xs)| && 0 <= j < |subsetSeqs(xs)| ==> ToSet(subsetSeqs(xs)[i]) != ToSet(subsetSeqs(xs)[j]);
+        }else{
+            assert xs == [xs[0]]+xs[1..];
+            subsetSeqsDistinct(xs);
+            subsetSeqToSetNotEqual(xs[1..]);
+            var rest := subsetSeqs(xs[1..]);
+            var mapped := Map((ss: seq<T>) => prepend(xs[0], ss), subsetSeqs(xs[1..]));
+            assert |mapped| == |rest|;
+            assert subsetSeqs(xs) == mapped + rest;
+            subsetSeqsContains(xs[1..]);
+            forall i,j | i != j && 0 <= i < |subsetSeqs(xs)| && 0 <= j < |subsetSeqs(xs)|
+                ensures ToSet(subsetSeqs(xs)[i]) != ToSet(subsetSeqs(xs)[j])
+            {
+                if i >= |rest| && j >= |rest| {
+
+                    assert ToSet(subsetSeqs(xs)[i]) != ToSet(subsetSeqs(xs)[j]);
+                }else if i < |rest| && j < |rest| {
+                    subsetSeqsDistinct(xs[1..]);
+                    forall m,n | m != n && 0 <= m < n < |mapped|
+                        ensures ToSet(mapped[m]) != ToSet(mapped[n])
+                    {
+                        assert mapped[m] == [xs[0]]+subsetSeqs(xs[1..])[m];
+                        assert mapped[n] == [xs[0]]+subsetSeqs(xs[1..])[n];
+                        assert subsetSeqs(xs[1..])[m] != subsetSeqs(xs[1..])[n];
+                        assert ToSet(subsetSeqs(xs[1..])[m]) != ToSet(subsetSeqs(xs[1..])[n]);
+                        assert ToSet(mapped[m]) == {xs[0]}+ToSet(subsetSeqs(xs[1..])[m]);
+                        assert ToSet(mapped[n]) == {xs[0]}+ToSet(subsetSeqs(xs[1..])[n]);
+                        assert subsetSeqs(xs[1..])[m] in subsetSeqs(xs[1..]);
+                        assert subsetSeqs(xs[1..])[n] in subsetSeqs(xs[1..]);
+                        setsNotEqualPlusOne(ToSet(subsetSeqs(xs[1..])[m]), ToSet(subsetSeqs(xs[1..])[n]), xs[0]);
+                    }
+
+                    assert ToSet(subsetSeqs(xs)[i]) != ToSet(subsetSeqs(xs)[j]);
+                }else{
+                    var x := xs[0];
+                    if i < |rest| {
+                        assert j >= |rest|;
+                        assert x in mapped[i];
+                        assert subsetSeqs(xs)[j] in subsetSeqs(xs[1..]);
+                        assert x !in subsetSeqs(xs)[j];
+                    }else{
+                        assert x in mapped[j];
+                        assert subsetSeqs(xs)[i] in subsetSeqs(xs[1..]);
+                        assert x !in subsetSeqs(xs)[i];
+                        assert j < |rest| && i >= |rest|;
+                    }
+                    assert ToSet(subsetSeqs(xs)[i]) != ToSet(subsetSeqs(xs)[j]);
+                }
+            }
+
+            assert forall i,j :: i != j && 0 <= i < |subsetSeqs(xs)| && 0 <= j < |subsetSeqs(xs)| ==> ToSet(subsetSeqs(xs)[i]) != ToSet(subsetSeqs(xs)[j]);
+        }
+    }
+
+    /*
+        filter (<|(p:ps) (subseqs (p:ps)))
+    */
+
+    function FindCCliqueNaive<Person(!new)(==)>(xs: seq<Person>): seq<seq<Person>>
+        requires distinct(xs)
+        ensures forall cs :: cs in FindCCliqueNaive(xs) ==> IsCelebrityClique(ToSet(cs), ToSet(xs))
+        ensures FindCCliqueNaive(xs) != [] ==> |FindCCliqueNaive(xs)| == 1
     {
         var people := ToSet(xs);
-        Filter((ss) => IsCelebrityClique(ToSet(ss),  people),subsetSeqs(xs))
+        var result := Filter((ss) => IsCelebrityClique(ToSet(ss),  people),subsetSeqs(xs));
+        assert forall cs :: cs in result ==> IsCelebrityClique(ToSet(cs), ToSet(xs));
+        // subsetSeqsDistinct(xs);
+        subsetSeqToSetNotEqual(xs);
+        assert |result| > 0 ==> |result| == 1 by {
+            if |result| > 1 {
+                FilterTargets((ss) => IsCelebrityClique(ToSet(ss),  people),subsetSeqs(xs));
+                var cs := result[0];
+                forall i | 1 < i < |result| 
+                    ensures ToSet(result[i]) == ToSet(cs)
+                {
+                    if ToSet(result[i]) != ToSet(cs) {
+                        CelebrityCliqueIsUnique(ToSet(cs), ToSet(result[i]), ToSet(xs));
+                    }
+                }
+                assert false;
+            }
+        }
+        result
     }
 
     predicate nonmember<Person(==)>(p: Person, cs: set<Person>) 
@@ -148,12 +327,157 @@ module CelebrityCliques {
         forall c :: c in cs ==> Knows(p, c) && !Knows(c, p)
     }
 
+    predicate member<Person(==)>(p: Person, cs: set<Person>, ps: set<Person>) 
+    {
+        forall x :: x in ps ==> Knows(x, p) && (Knows(p,x) <==> x in cs)
+    }
+
+    lemma opps1<Person(==)>(p: Person, cs: set<Person>, ps: set<Person>)
+        requires p in ps
+        requires cs <= ps
+        requires nonmember(p, cs)
+        ensures !member(p, cs, ps)
+    {
+    }
+
+    // lemma opps4<Person(==)>(p: Person, cs: set<Person>, ps: set<Person>)
+    //     requires p in ps
+    //     requires cs <= ps
+    //     requires !nonmember(p, cs)
+    //     ensures member(p, cs, ps)
+    // {
+    // }
+
+    lemma opps2<Person(==)>(p: Person, cs: set<Person>, ps: set<Person>)
+        requires p in ps
+        requires cs <= ps
+        requires member(p, cs, ps)
+        ensures !nonmember(p, cs)
+    {
+    }
+
+    // lemma {:isolate_assertions} opps3<Person(==)>(p: Person, cs: set<Person>, ps: seq<Person>)
+    //     requires |ps| > 1
+    //     requires p == ps[0]
+    //     requires cs <= ToSet(ps)
+    //     requires forall q: Person :: q in ps ==> Knows(q,q)
+    //     requires IsCelebrityClique(cs, ToSet(ps[1..]))
+    //     requires !member(p, cs, ToSet(ps))
+    //     ensures nonmember(p, cs)
+    // {
+    //     var x :| x in ps && (!Knows(x, p) || (Knows(x, p) && !(Knows(p,x) <==> x in cs)));
+    //     if !Knows(x, p) {
+    //         assert x != p;
+    //         assert x in ps[1..];
+    //         if !nonmember(p, cs) {
+    //             var c :| c in cs && (!Knows(p, c) || Knows(c, p));
+    //             if !Knows(p, c) {
+    //                 assert false;
+    //             }else if Knows(c, p) {
+
+    //                 assert false;
+    //             }
+    //             assert false;
+    //         }
+
+    //         assert nonmember(p, cs);
+    //     }else{
+
+    //         if !nonmember(p, cs) {
+    //             assert false;
+    //         }
+    //         assert nonmember(p, cs);
+    //     }
+    // }
+    lemma opps5<Person(==)>(p: Person, cs: set<Person>, ps: set<Person>)
+        requires p in ps
+        requires cs <= ps
+        requires cs == {}
+        requires !member(p, cs, ps)
+        ensures nonmember(p, cs)
+    {
+        var x :| x in ps && (!Knows(x, p) || (Knows(x, p) && !(Knows(p,x) <==> x in cs)));
+        if !Knows(x, p) {
+
+            assert nonmember(p, cs);
+        }else{
+
+            assert nonmember(p, cs);
+        }
+    }
+
+    // lemma NonMemberSimplification<Person(==)>(xs: seq<Person>, people: seq<Person>) 
+    //     requires |xs| > 1
+    //     requires ToSet(xs) <= ToSet(people)
+    //     ensures IsCelebrityClique(ToSet(xs),  ToSet(people)) == IsCelebrityClique(ToSet(xs[1..]), ToSet(people)) && nonmember(xs[0], ToSet(xs[1..]))
+    // {
+
+    // }
+
+    // lemma testMember<Person>(p: Person, ps: seq<Person>)
+    //     requires p in ps
+    //     requires forall x :: x in ToSet(ps) ==> Knows(x, p)
+    //     ensures member(p, ToSet([]), ToSet(ps))
+    // {}
+
+    lemma testnonMember<Person>(p: Person, ps: seq<Person>)
+        requires p in ps
+        ensures nonmember(p, ToSet([]))
+    {}
+
+    /*
+        ccliques [] = [[]]
+        ccliques (p:ps) == map (p:) (filter (member p ps) css) ++
+                           filter (nonmember p) css
+                           where css = ccliques ps
+    */
+    function ccliques<Person(!new)(==)>(ps: seq<Person>): seq<seq<Person>> 
+        requires distinct(ps)
+        ensures 1 <= |ccliques(ps)|
+        ensures [] in ccliques(ps)
+        ensures forall cs :: cs in ccliques(ps) ==> ToSet(cs) <= ToSet(ps)
+        ensures forall cs :: cs in ccliques(ps) && |cs| > 0 ==> IsCelebrityClique(ToSet(cs), ToSet(ps))
+    {
+        if ps == [] then 
+            [[]]
+        else
+            var p := ps[0];
+            var css := ccliques(ps[1..]);
+            var left := Map(pss => prepend(p, pss), Filter(cs => member(p, ToSet(cs), ToSet(ps)), css));
+            var right := Filter(cs => nonmember(p, ToSet(cs)), css);
+            assert [] in css;
+            // testnonMember(p, ps);
+            FilterHas(cs => nonmember(p, ToSet(cs)), css, []);
+            assert [] in right;
+            assert ps == [p]+ps[1..];
+            ToSetConcat([p], ps[1..]);
+            assert ToSet(ps[1..]) <= ToSet(ps);
+            FilteredInXS(cs => nonmember(p, ToSet(cs)), css);
+            var leftPre := Filter(cs => member(p, ToSet(cs), ToSet(ps)), css);
+            FilteredInXS(cs => member(p, ToSet(cs), ToSet(ps)), css);
+            forall cs | cs in left
+                ensures ToSet(cs) <= ToSet(ps)
+            {
+                var i :| 0 <= i < |left| && left[i] == cs;
+                var m :| 0 <= m < |leftPre| && prepend(p, leftPre[m]) == cs;
+                ToSetConcat([p], leftPre[m]);
+                assert ToSet(cs) == {p} + ToSet(leftPre[m]);
+            }
+            forall cs | cs in right
+                ensures ToSet(cs) <= ToSet(ps)
+            {
+                
+            }
+            forall cs | cs in left+right && |cs| > 0
+                ensures IsCelebrityClique(ToSet(cs), ToSet(ps))
+            {}
+            left + right
+    }
+
     lemma mapTest<T,R>(xs: seq<T>, f: T -> R)
         requires |xs| != 0
         ensures Map(f, xs)[0] == f(xs[0])
     {
-
- 
         // assert |xs| != 0;
         // assert |xs| > 0;
         // assert |xs| == |Map(f, xs)|;
