Pearls/SeqFunctions.dfy
@@ -36,6 +36,12 @@ function Filter<T>(f: (T -> bool), xs: seq<T>): (result: seq<T>)
     else (if f(xs[0]) then [xs[0]] else []) + Filter(f, xs[1..])
   }
 
+  lemma FilterHas<T>(f: T-> bool, xs: seq<T>, x: T)
+    requires x in xs
+    requires f(x)
+    ensures x in Filter(f, xs)
+  {}
+
   /* Filtering a sequence is distributive over concatenation. That is, concatenating two sequences 
      and then using "Filter" is the same as using "Filter" on each sequence separately, and then 
      concatenating the two resulting sequences. */
@@ -101,4 +107,164 @@ function Filter<T>(f: (T -> bool), xs: seq<T>): (result: seq<T>)
         assert Filter(Conj(f,g), xs) == Filter(f, Filter(g, xs));
     }
   }
+
+  lemma FilteredInXS<T(!new)>(f: T -> bool, xs: seq<T>)
+    ensures forall xx :: xx in Filter(f, xs) ==> xx in xs
+  {}
+
+  lemma FilterTargets<T(!new)>(f: T -> bool, xs: seq<T>)
+    requires |Filter(f, xs)| > 1
+    ensures exists i,j, m,n :: i != j && 0 <= i < j < |Filter(f, xs)| && m != n && 0 <= m < n < |xs| && f(xs[m]) && xs[m] == Filter(f, xs)[i] && f(xs[n]) && xs[n] == Filter(f, xs)[j]
+  {
+    assert |xs| >= |Filter(f, xs)|;
+    assert xs == [xs[0]]+xs[1..];
+    assert xs == [xs[0]]+[xs[1]]+xs[2..];
+    assert xs[1..][1..] == xs[2..];
+    // FilteredInXS(f, xs);
+    FilteredInXS(f, xs[1..]);
+    FilteredInXS(f, xs[2..]);
+    if |Filter(f, xs)| == 2 {
+      assert Filter(f,xs)[0] in xs;
+      assert Filter(f,xs)[1] in xs;
+      if f(xs[0]) {
+        calc {
+          Filter(f, xs);
+          [xs[0]]+Filter(f, xs[1..]);
+        }
+        assert Filter(f,xs)[1] in Filter(f, xs[1..]);
+        assert Filter(f, xs)[0] == xs[0];
+        assert Filter(f,xs)[1] in Filter(f, xs[1..]);
+        var j :| 0 <= j < |xs[1..]|  && Filter(f, xs)[1] == xs[1..][j];
+        assert Filter(f, xs)[1] == xs[j+1];
+      }else if f(xs[1]) {
+        assert Filter(f, xs)[0] == xs[1];
+        calc {
+          Filter(f, xs);
+          [] + Filter(f, xs[1..]);
+          [xs[1]]+Filter(f, xs[1..][1..]);
+          [xs[1]]+Filter(f, xs[2..]);
+        }
+        assert Filter(f,xs)[1] in Filter(f, xs[2..]);
+        var j :| 0 <= j < |xs[2..]|  && Filter(f, xs)[1] == xs[2..][j];
+        assert Filter(f, xs)[1] == xs[j+2];
+      }else{
+        FilterTargets(f, xs[2..]);
+      }
+    }else{
+      // FilterTargets(f, xs[1..]);
+      if f(xs[0]) {
+        assert Filter(f, xs)[0] == xs[0];
+        calc {
+          Filter(f, xs);
+          [xs[0]]+Filter(f, xs[1..]);
+        }
+        assert Filter(f,xs)[1] in Filter(f, xs[1..]);
+        var j :| 0 <= j < |xs[1..]|  && Filter(f, xs)[1] == xs[1..][j];
+        assert Filter(f, xs)[1] == xs[j+1];
+      }else if f(xs[1]) {
+        calc {
+          Filter(f, xs);
+          [] + Filter(f, xs[1..]);
+          [xs[1]]+Filter(f, xs[1..][1..]);
+          [xs[1]]+Filter(f, xs[2..]);
+        }
+        assert Filter(f, xs)[0] == xs[1];
+        assert Filter(f,xs)[1] in Filter(f, xs[2..]);
+        var j :| 0 <= j < |xs[2..]|  && Filter(f, xs)[1] == xs[2..][j];
+        assert Filter(f, xs)[1] == xs[j+2];
+      }else{
+        calc {
+          Filter(f, xs);
+          [] + Filter(f, xs[1..]);
+          [] + [] + Filter(f, xs[1..][1..]);
+        }
+        FilterTargets(f, xs[2..]);
+
+      }
+    }
+  }
+
+  // lemma FilterTargeted<T(!new)(==)>(f: T->bool, xs: seq<T>, i: nat, j: nat)
+  //   requires |Filter(f, xs)| > 1
+  //   requires i < j < |Filter(f, xs)|
+  //   ensures exists m,n :: m != n && 0 <= m < n < |xs| && Filter(f,xs)[i] == xs[m] && Filter(f, xs)[j] == xs[n] 
+  // {
+  //   // FilterTargets(f, xs);
+  //   assert |xs| >= |Filter(f, xs)|;
+  //   assert xs == [xs[0]]+xs[1..];
+  //   assert xs == [xs[0]]+[xs[1]]+xs[2..];
+  //   assert xs[1..][1..] == xs[2..];
+  //   FilteredInXS(f, xs);
+  //   FilteredInXS(f, xs[1..]);
+  //   FilteredInXS(f, xs[2..]);
+
+  //   if |Filter(f, xs)| == 2 {
+  //     assert Filter(f,xs)[0] in xs;
+  //     assert Filter(f,xs)[1] in xs;
+  //     assert i == 0;
+  //     assert j == 1;
+  //     if f(xs[0]) {
+  //       calc {
+  //         Filter(f, xs);
+  //         [xs[0]]+Filter(f, xs[1..]);
+  //       }
+  //       assert Filter(f,xs)[1] in Filter(f, xs[1..]);
+  //       assert Filter(f, xs)[0] == xs[0];
+  //       assert Filter(f,xs)[1] in Filter(f, xs[1..]);
+  //       var n :| 0 <= n < |xs[1..]|  && Filter(f, xs)[1] == xs[1..][n];
+  //       assert Filter(f, xs)[1] == xs[n+1];
+  //     }else if f(xs[1]) {
+  //       assert Filter(f, xs)[0] == xs[1];
+  //       calc {
+  //         Filter(f, xs);
+  //         [] + Filter(f, xs[1..]);
+  //         [xs[1]]+Filter(f, xs[1..][1..]);
+  //         [xs[1]]+Filter(f, xs[2..]);
+  //       }
+  //       assert Filter(f,xs)[1] in Filter(f, xs[2..]);
+  //       var n :| 0 <= n < |xs[2..]|  && Filter(f, xs)[1] == xs[2..][n];
+  //       assert Filter(f, xs)[1] == xs[n+2];
+  //     }else{
+  //       FilterTargeted(f, xs[2..], i,j);
+  //     }
+  //   }else{
+  //     var fs := Filter(f, xs);
+  //     if i == 0 {
+
+  //     }else{
+
+  //     }
+  //     // FilterTargets(f, xs[1..]);
+  //     // if f(xs[0]) {
+  //     //   assert Filter(f, xs)[0] == xs[0];
+  //     //   calc {
+  //     //     Filter(f, xs);
+  //     //     [xs[0]]+Filter(f, xs[1..]);
+  //     //   }
+  //     //   assert Filter(f,xs)[1] in Filter(f, xs[1..]);
+  //     //   var n :| 0 <= n < |xs[1..]|  && Filter(f, xs)[1] == xs[1..][n];
+  //     //   assert Filter(f, xs)[1] == xs[n+1];
+  //     // }else if f(xs[1]) {
+  //     //   calc {
+  //     //     Filter(f, xs);
+  //     //     [] + Filter(f, xs[1..]);
+  //     //     [xs[1]]+Filter(f, xs[1..][1..]);
+  //     //     [xs[1]]+Filter(f, xs[2..]);
+  //     //   }
+  //     //   assert Filter(f, xs)[0] == xs[1];
+  //     //   assert Filter(f,xs)[1] in Filter(f, xs[2..]);
+  //     //   var n :| 0 <= n < |xs[2..]|  && Filter(f, xs)[1] == xs[2..][n];
+  //     //   assert Filter(f, xs)[1] == xs[n+2];
+  //     // }else{
+  //     //   calc {
+  //     //     Filter(f, xs);
+  //     //     [] + Filter(f, xs[1..]);
+  //     //     [] + [] + Filter(f, xs[1..][1..]);
+  //     //   }
+  //     //   FilterTargeted(f, xs[2..], i,j);
+
+  //     // }
+  //   }
+    
+  // }
 }
